theories/sim/adequacy.v
@@ -9,43 +9,44 @@ Set Default Proof Using "Type".
 
 Inductive behavior := | Term (v: value) | Stuck | Diverges.
 
-Inductive behaviors
-  (step: expr * config → expr * config → Prop)
-  (cfg: expr * config) : behavior → Prop :=
+Inductive behaviors (fns: fn_env)
+  (step: fn_env → expr * state → expr * state → Prop)
+  (cfg: expr * state) : behavior → Prop :=
 | behaviors_term v
     (TERMINAL: to_result cfg.1 = Some (ValR v)) :
-    behaviors step cfg (Term v)
+    behaviors fns step cfg (Term v)
 | behaviors_stuck
     (NT: ¬ terminal cfg.1)
-    (NS: ∀ cfg', ¬ step cfg cfg') :
-    behaviors step cfg Stuck
+    (NS: ∀ cfg', ¬ step fns cfg cfg') :
+    behaviors fns step cfg Stuck
 (* | behaviors_diverges
     (DIV: diverges step cfg) :
     behaviors step cfg Diverges *)
 | behaviors_step cfg' ov
-    (STEP: step cfg cfg')
-    (NEXT: behaviors step cfg' ov):
-    behaviors step cfg ov
+    (STEP: step fns cfg cfg')
+    (NEXT: behaviors fns step cfg' ov):
+    behaviors fns step cfg ov
 .
 
 (* If c1 ->* c2 -b-> v then c1 -b-> v *)
-Lemma rtc_step_behavior step c1 c2 v
-  (STEPS: rtc step c1 c2) (BEH: behaviors step c2 v):
-  behaviors step c1 v.
+Lemma rtc_step_behavior fns step c1 c2 v
+  (STEPS: rtc (step fns) c1 c2) (BEH: behaviors fns step c2 v):
+  behaviors fns step c1 v.
 Proof.
   induction STEPS as [|c1 c2 c3 S1 S2 IH]; [done|]. specialize (IH BEH).
   econstructor 3; eauto.
 Qed.
 
-Lemma sim_adequacy (cfg_src cfg_tgt: expr * config)
-  (WFS: Wf cfg_src.2) (WFT: Wf cfg_tgt.2) (NO_UB: no_UB cfg_src)
-  (SIM: sim cfg_src cfg_tgt) :
-  behaviors tstep cfg_tgt <1= behaviors tstep cfg_src.
+Lemma sim_adequacy fns fnt (cfg_src cfg_tgt: expr * state)
+  (NO_UB: no_UB fns cfg_src)
+  (SIM: sim fns fnt cfg_src cfg_tgt) :
+  behaviors fns tstep cfg_tgt <1= behaviors fnt tstep cfg_src.
 Proof.
-  intros ov BEH. revert cfg_src WFS WFT NO_UB SIM.
+  intros ov BEH. revert cfg_src NO_UB SIM.
   induction BEH as [cfg_tgt(* |cfg_tgt *)|cfg_tgt v|cfg_tgt cfg_tgt' ov STEP BEH IH];
-    intros cfg_src WFS WFT NO_UB SIM.
-  - punfold SIM. destruct (SIM WFS WFT) as [? (* ? *) TERM ?]; [naive_solver|].
+    intros cfg_src NO_UB SIM.
+  - punfold SIM.
+    (* destruct (SIM WFS WFT) as [? (* ? *) TERM ?]; [naive_solver|].
     destruct TERM as (eσ2 & TS & TERM' & VAL); [by eexists|].
     apply (rtc_step_behavior _ _ _ _ TS).
     constructor. by apply VAL.
@@ -67,5 +68,5 @@ Proof.
     + by apply (tstep_wf _ _ STEP).
     + clear -STEP' NO_UB. induction STEP'. done.
       apply IHSTEP'. admit.
-    + by inversion TS'.
+    + by inversion TS'. *)
 Abort.
