theories/sim/global.v
@@ -8,7 +8,7 @@ CoInductive diverges
 | DivergeStep cfg' (STEP: step cfg cfg') (DIV: diverges step cfg') .
 
 Definition sim_expr_terminal (e1 e2: expr) :=
-  ∀ v2, to_val e2 = Some v2 → to_val e1 = Some v2.
+  ∀ v2, to_value e2 = Some v2 → to_value e1 = Some v2.
 Instance sim_expr_terminal_po : PreOrder sim_expr_terminal.
 Proof.
   constructor.
@@ -16,35 +16,38 @@ Proof.
   - move => e1 e2 e3 S1 S2 v3 /S2 /S1 //.
 Qed.
 
-Notation SIM_CONFIG := (expr * config → expr * config → Prop)%type.
+Notation SIM_CONFIG := (expr * state → expr * state → Prop)%type.
 
 (* This is a simulation between two expressions without any interference.
   It corresponds to a sequential simulation. *)
 
-Record sim_base (sim: SIM_CONFIG) (eσ1_src eσ1_tgt: expr * config) : Prop := mkSimBase {
+Section sim.
+Variable (fns fnt: fn_env).
+
+Record sim_base (sim: SIM_CONFIG) (eσ1_src eσ1_tgt: expr * state) : Prop := mkSimBase {
   (* (1) If [eσ1_tgt] gets stuck, [eσ1_src] can also get stuck. *)
   sim_stuck :
-    stuck eσ1_tgt.1 eσ1_tgt.2 → ∃ eσ2_src,
-    eσ1_src ~t~>* eσ2_src ∧ stuck eσ2_src.1 eσ2_src.2 ;
+    stuck (Λ:= bor_lang fnt) eσ1_tgt.1 eσ1_tgt.2 → ∃ eσ2_src,
+    eσ1_src ~{fns}~>* eσ2_src ∧ stuck (Λ:= bor_lang fns) eσ2_src.1 eσ2_src.2 ;
   (* (2) If [eσ1_tgt] diverges, then [eσ1_src] diverges. *)
   (* sim_diverges : diverges tstep eσ1_tgt → diverges tstep eσ1_src ; *)
   (* (3) If [eσ1_tgt] is terminal, then [eσ1_src] terminates with some steps. *)
   sim_terminal :
     terminal eσ1_tgt.1 → ∃ eσ2_src,
-    eσ1_src ~t~>* eσ2_src ∧ terminal eσ2_src.1 ∧ sim_expr_terminal eσ2_src.1 eσ1_tgt.1;
+    eσ1_src ~{fns}~>* eσ2_src ∧ terminal eσ2_src.1 ∧ sim_expr_terminal eσ2_src.1 eσ1_tgt.1;
   (* (4) If [eσ1_tgt] steps to [eσ2_tgt] with 1 step,
        then exists [eσ2_src] s.t. [eσ1_src] steps to [eσ2_src] with * step. *)
   sim_step :
-    ∀ eσ2_tgt, eσ1_tgt ~t~> eσ2_tgt → ∃ eσ2_src,
-      eσ1_src ~t~>* eσ2_src ∧ sim eσ2_src eσ2_tgt;
+    ∀ eσ2_tgt, eσ1_tgt ~{fnt}~> eσ2_tgt → ∃ eσ2_src,
+      eσ1_src ~{fns}~>* eσ2_src ∧ sim eσ2_src eσ2_tgt;
 }.
 
-Definition no_UB (eσ: expr * config) : Prop :=
-  ¬ (∀ eσ', eσ ~t~>* eσ' → stuck eσ'.1 eσ'.2).
+Definition no_UB (eσ: expr * state) : Prop :=
+  ¬ (∀ eσ', eσ ~{fns}~>* eσ' → stuck (Λ:= bor_lang fns) eσ'.1 eσ'.2).
 
 (* Generator for the actual simulation *)
 Definition _sim
-  (sim : SIM_CONFIG) (eσ1_src eσ1_tgt: expr * config) : Prop :=
+  (sim : SIM_CONFIG) (eσ1_src eσ1_tgt: expr * state) : Prop :=
   Wf eσ1_src.2 → Wf eσ1_tgt.2 →
   (* If [eσ1_src] gets UB, we can have UB in the target, thus any [eσ1_tgt] is
       acceptable. Otherwise ... *)
@@ -60,5 +63,7 @@ Qed.
 
 (* Global simulation *)
 Definition sim : SIM_CONFIG := paco2 _sim bot2.
+
+End sim.
 
 Hint Resolve _sim_mono: paco.
