theories/sim/local.v
@@ -9,7 +9,7 @@ Section local.
 Context {A: ucmraT}.
 Variable (wsat: A → state → state → Prop).
 Variable (vrel: A → expr → expr → Prop).
-Variable (fns_src fns_tgt: fn_env).
+Variable (fns fnt: fn_env).
 
 (* TODO: encode what it means for the context to not contain our private tags! *)
 (* TODO: how do we know we're at the top of the stack? *)
@@ -18,24 +18,27 @@ Inductive _sim_local_body
   (r: A) : expr → state → expr → state → Prop :=
 (* If src is stuck, then anything is related *)
 | sim_local_body_stuck e_src σ_src e_tgt σ_tgt
-    (STUCK: stuck e_src (mkConfig fns_src σ_src))
+    (STUCK: stuck (Λ:=bor_lang fns) e_src σ_src)
     : _sim_local_body sim_local_body r e_src σ_src e_tgt σ_tgt
 (* If tgt makes 1 step, src can make some step *)
 | sim_local_body_step e_src σ_src e_tgt σ_tgt
-    (STEP: ∀ r_f e_tgt' cfg_tgt'
+    (STEP: ∀ r_f e_tgt' σ_tgt'
       (* for any frame r_f that is compatible with our resource r and has world satisfaction *)
       (VALID: ✓ (r_f ⋅ r)) (WSAT: wsat (r_f ⋅ r) σ_src σ_tgt)
       (* if tgt can locally make 1 step *)
-      (STEPT: (e_tgt, (mkConfig fns_tgt σ_tgt)) ~t~> (e_tgt', cfg_tgt')),
+      (STEPT: (e_tgt, σ_tgt) ~{fnt}~> (e_tgt', σ_tgt')),
       (* then we locally can makes some step and pick a new resource r' *)
-      ∃ e_src' cfg_src' r',
-        (e_src, (mkConfig fns_src σ_src)) ~t~>* (e_src', cfg_src') ∧
-        ✓ (r_f ⋅ r') ∧ wsat (r_f ⋅ r') cfg_src'.(cst) cfg_tgt'.(cst) ∧
-        sim_local_body r' e_src' cfg_src'.(cst) e_tgt' cfg_tgt'.(cst))
+      ∃ e_src' σ_src' r',
+        (e_src, σ_src) ~{fns}~>* (e_src', σ_src') ∧
+        ✓ (r_f ⋅ r') ∧ wsat (r_f ⋅ r') σ_src' σ_tgt' ∧
+        sim_local_body r' e_src' σ_src' e_tgt' σ_tgt')
     : _sim_local_body sim_local_body r e_src σ_src e_tgt σ_tgt
 (* If tgt prepares to make a call to [name], src should be able to make the same
   call. Here we do not want to step into the call of [name], but to step over it. *)
-| sim_local_body_step_over_call K_src K_tgt fid e_src e_tgt el_tgt σ_src σ_tgt
+| sim_local_body_step_over_call
+    (K_src: list (ectxi_language.ectx_item (bor_ectxi_lang fns)))
+    (K_tgt: list (ectxi_language.ectx_item (bor_ectxi_lang fnt)))
+    fid e_src e_tgt el_tgt σ_src σ_tgt
     (CALLTGT: e_tgt = fill K_tgt (Call #[ScFnPtr fid] el_tgt))
     (STEPOVER: ∀ r_f
         (* for any frame r_f that is compatible with our resource r and has world satisfaction *)
@@ -44,40 +47,39 @@ Inductive _sim_local_body
         (* tgt is ready to make a call of [name] *)
         (VTGT : Forall (λ ei, is_Some (to_value ei)) el_tgt),
         (* then src is also ready to make a call of [name] *)
-        ∃ el_src cfg_src rc rv,
-        (e_src, (mkConfig fns_src σ_src)) ~t~>*
-          (fill K_src (Call #[ScFnPtr fid] el_src), cfg_src) ∧
+        ∃ el_src σ1_src rc rv,
+        (e_src, σ_src) ~{fns}~>* (fill K_src (Call #[ScFnPtr fid] el_src), σ1_src) ∧
         Forall (λ ei, is_Some (to_value ei)) el_src ∧
         (* and we can pick a resource [rv] for the arguments *)
-        ✓ (r_f ⋅ (rc ⋅ rv)) ∧ wsat (r_f ⋅ (rc ⋅ rv)) cfg_src.(cst) σ_tgt ∧
+        ✓ (r_f ⋅ (rc ⋅ rv)) ∧ wsat (r_f ⋅ (rc ⋅ rv)) σ1_src σ_tgt ∧
         (* [rv] justifies the arguments *)
         Forall2 (vrel rv) el_src el_tgt ∧
         (* and after the call our context can continue *)
-        (∀ r_f' r' v_src v_tgt cfg_src' cfg_tgt'
+        (∀ r_f' r' v_src v_tgt σ_src' σ_tgt'
           (* For any new resource r' and frame r_f' that are compatible with
              our local resource r and has world satisfaction *)
           (VALID': ✓ (r_f' ⋅ (rc ⋅ r')))
-          (WSAT' : wsat (r_f ⋅ (rc ⋅ r')) cfg_src'.(cst) cfg_tgt'.(cst))
+          (WSAT' : wsat (r_f ⋅ (rc ⋅ r')) σ_src' σ_tgt')
           (* and the returned values are related w.r.t. (r ⋅ r' ⋅ r_f) *)
           (VRET  : vrel r' (Val v_src) (Val v_tgt)),
           sim_local_body (rc ⋅ r')
-                      (fill K_src (Val v_src)) cfg_src'.(cst)
-                      (fill K_tgt (Val v_tgt)) cfg_tgt'.(cst)))
+                      (fill K_src (Val v_src)) σ_src'
+                      (fill K_tgt (Val v_tgt)) σ_tgt'))
     : _sim_local_body sim_local_body r e_src σ_src e_tgt σ_tgt
 (* If tgt prepares to end, src also prepares to end *)
 | sim_local_body_end_call v_src σ_src v_tgt σ_tgt e_src e_tgt
     (ESRC: e_src = EndCall (Val v_src))
     (ETGT: e_tgt = EndCall (Val v_tgt))
-    (END: ∀ r_f cfg_tgt'
+    (END: ∀ r_f eσ_tgt'
         (VALID: ✓ (r_f ⋅ r))
         (WSAT : wsat (r_f ⋅ r) σ_src σ_tgt)
         (* if tgt can end call *)
-        (ETGT: (EndCall (Val v_tgt), (mkConfig fns_tgt σ_tgt)) ~t~> cfg_tgt'),
+        (ETGT: (EndCall (Val v_tgt), σ_tgt) ~{fnt}~> eσ_tgt'),
         (* then src can also end call *)
-        ∃ cfg_src' r',
-        (EndCall (Val v_src), (mkConfig fns_src σ_tgt)) ~t~> cfg_src' ∧
+        ∃ eσ_src' r',
+        (EndCall (Val v_src), σ_src) ~{fns}~> eσ_src' ∧
         (* and re-establish wsat *)
-        ✓ (r_f ⋅ r') ∧ wsat (r_f ⋅ r') cfg_src'.2.(cst) cfg_tgt'.2.(cst) ∧
+        ✓ (r_f ⋅ r') ∧ wsat (r_f ⋅ r') eσ_src'.2 eσ_tgt'.2 ∧
         (* and the returned values are related *)
         vrel r' (Val v_src) (Val v_tgt))
     : _sim_local_body sim_local_body r e_src σ_src e_tgt σ_tgt
@@ -147,8 +149,8 @@ Definition sim_local_fun (fn_src fn_tgt : function) : Prop :=
     sim_local_body r (InitCall e_src) σ_src (InitCall e_tgt) σ_tgt.
 
 Definition sim_local_funs : Prop :=
-  ∀ name fn_src, fns_src !! name = Some fn_src → ∃ fn_tgt,
-    fns_tgt !! name = Some fn_tgt ∧ sim_local_fun fn_src fn_tgt.
+  ∀ name fn_src, fns !! name = Some fn_src → ∃ fn_tgt,
+    fnt !! name = Some fn_tgt ∧ sim_local_fun fn_src fn_tgt.
 
 End local.
 
